Recast triR to record how many steps are taken by left argument
This makes simulation result stronger as we know that in all cases
either the left argument moves, or a different well-founded relation
decreases (size of outgoing queues in network).

projection/proofs/to_cake/abstractCompilationScript.sml
@@ -1,7 +1,9 @@
 open HolKernel Parse boolLib bossLib;
 
-open relationTheory
+open relationTheory arithmeticTheory
 val _ = new_theory "abstractCompilation";
+
+fun SRULE ths = SIMP_RULE (srw_ss()) ths
 
 Definition postcloud_def:
   postcloud c sR tR s t ⇔ tR꙳ (c s) t ∧ ∀s'. sR s s' ⇒ tR⁺ t (c s')
@@ -63,72 +65,341 @@ Proof
 QED
 
 Definition triR_def:
-  triR R e1 e2 ⇔ ∃e. R꙳ e1 e ∧ R꙳ e2 e
+  triR R n e1 e2 ⇔ ∃e. NRC R n e1 e ∧ R꙳ e2 e
 End
 
-Theorem RTC_triR:
-  R꙳ a b ⇒ triR R a b
+Definition tcdistance_def:
+  tcd R a b = (@n. NRC R n a b) - 1
+End
+
+Theorem TC_triR0:
+  R⁺ a b ⇒ ∃n. triR R (n + 1) a b
 Proof
-  simp[triR_def] >> metis_tac[RTC_REFL]
+  simp[triR_def, TC_eq_NRC, ADD1] >> metis_tac[RTC_REFL]
 QED
 
+Theorem TC_triR[local] =
+        TC_triR0 |> Q.GENL[‘R’, ‘a’, ‘b’]
+                 |> SRULE [GSYM RIGHT_EXISTS_IMP_THM, SKOLEM_THM]
+
+val tcd_def = new_specification("tcd_def", ["tcd"], TC_triR)
+
 Theorem triR_one_step_each:
-  R a0 a ∧ R b0 b ∧ triR R a b ⇒ triR R a0 b0
+  R a0 a ∧ R b0 b ∧ triR R n a b ⇒ triR R (n + 1) a0 b0
 Proof
-  simp[triR_def] >> metis_tac[RTC_RULES]
+  simp[triR_def] >> strip_tac >> ONCE_REWRITE_TAC [ADD_COMM] >>
+  irule_at Any NRC_ADD_I >> simp[] >> metis_tac[RTC_RULES]
 QED
 
 Theorem triR_step1:
-  R a0 a ∧ triR R a b ⇒ triR R a0 b
+  R a0 a ∧ triR R n a b ⇒ triR R (n + 1) a0 b
+Proof
+  simp[triR_def] >> strip_tac >> ONCE_REWRITE_TAC [ADD_COMM] >>
+  irule_at Any NRC_ADD_I >> simp[] >> metis_tac[RTC_RULES]
+QED
+
+Theorem triR_steps10:
+  R꙳ a0 a ∧ triR R n a b ⇒ ∃d. triR R (n + d) a0 b
+Proof
+  simp[triR_def] >> strip_tac >> irule_at Any NRC_ADD_I >>
+  ntac 2 (first_assum $ irule_at Any) >> metis_tac[RTC_eq_NRC]
+QED
+
+Theorem RTC_steps =
+        RTC_eq_NRC |> iffLR
+                   |> SRULE [GSYM RIGHT_EXISTS_IMP_THM, SKOLEM_THM]
+
+val rtd_def = new_specification("rtd_def", ["rtd"], RTC_steps)
+
+Theorem triR_steps1:
+  R꙳ a0 a ∧ triR R n a b ⇒ triR R (n + rtd R a0 a) a0 b
+Proof
+  strip_tac >> drule rtd_def >> gs[triR_def] >>
+  metis_tac[NRC_ADD_I, ADD_COMM]
+QED
+
+Theorem triR_REFL[simp]:
+  ∀x. triR R 0 x x
+Proof
+  simp[triR_def]
+QED
+
+Theorem triR_step1R:
+  triR R n a b ∧ R b0 b ⇒ triR R n a b0
 Proof
   simp[triR_def] >> metis_tac[RTC_RULES]
 QED
 
-Theorem triR_steps1:
-  R꙳ a0 a ∧ triR R a b ⇒ triR R a0 b
+Theorem triR_stepsR:
+  R꙳ b0 b ∧ triR R n a b ⇒ triR R n a b0
 Proof
   simp[triR_def] >> metis_tac[RTC_CASES_RTC_TWICE]
 QED
 
-Theorem triR_RTC_each:
-  R꙳ a0 a ∧ R꙳ b0 b ∧ triR R a b ⇒ triR R a0 b0
+CoInductive mayloop:
+  ∀t0 t. mayloop tR t ∧ tR t0 t ⇒ mayloop tR t0
+End
+
+Theorem RC_mayloop[simp]:
+  ∀x. mayloop (RC R) x
 Proof
- metis_tac[triR_def, RTC_CASES_RTC_TWICE]
+  ‘∀x. K T x ⇒ mayloop (RC R) x’ suffices_by simp[] >>
+  ho_match_mp_tac mayloop_coind >> simp[EXISTS_OR_THM, RC_DEF]
 QED
 
-Theorem triR_REFL[simp]:
-  ∀x. triR R x x
+Definition mustloop_def:
+  mustloop R x ⇔ ∀y. RTC R x y ⇒ ∃z. R y z
+End
+
+Theorem mustloop_mayloop:
+  ∀x. mustloop R x ⇒ mayloop R x
 Proof
-  gen_tac >> simp[triR_def] >> irule_at Any RTC_REFL
+  ho_match_mp_tac mayloop_coind >> rw[] >>
+  rename [‘mustloop R x’] >>
+  ‘∃y. R x y’ by metis_tac[RTC_REFL, mustloop_def] >>
+  ‘∀z. R꙳ y z ⇒ R꙳ x z’ by metis_tac[RTC_RULES] >>
+  ‘mustloop R y’ by metis_tac[mustloop_def] >> metis_tac[]
 QED
 
-Theorem triR_SYM:
-  ∀x y. triR R x y = triR R y x
+Theorem det_term_xor_mayloop:
+  (∀t0 t1 t2. tR t0 t1 ∧ tR t0 t2 ⇒ t1 = t2) ⇒
+  ∀t0. ((∃t. nf tR t ∧ RTC tR t0 t) ⇔ ¬mayloop tR t0)
 Proof
-  simp[triR_def] >> metis_tac[]
+  strip_tac >> simp[FORALL_AND_THM, EQ_IMP_THM, PULL_EXISTS] >> conj_tac
+  >- (Induct_on ‘RTC’ >> rw[]
+      >- (gs[nf_def] >> simp[Once mayloop_cases]) >>
+      gs[] >> simp[Once mayloop_cases] >> metis_tac[]) >>
+  CONV_TAC (BINDER_CONV CONTRAPOS_CONV) >> simp[] >>
+  ho_match_mp_tac mayloop_coind >> rw[] >>
+  gs[nf_def] >> metis_tac[RTC_RULES]
 QED
 
-
-Theorem triR_forward_simulation_has_all_terminations:
-  simulates simR sR (triR tR) ∧ CR tR ∧
-  (∀s t. nf sR s ∧ simR s t ⇒ ∃tt. nf tR tt ∧ tR꙳ t tt ∧ simR s tt) ⇒
-  ∀s0 s t0.
-    sR꙳ s0 s ∧ nf sR s ∧ simR s0 t0 ⇒
-    ∃t.
-      tR꙳ t0 t ∧ nf tR t ∧ simR s t
+Theorem det_may_EQ_mustloop:
+  (∀x y1 y2. R x y1 ∧ R x y2 ⇒ y1 = y2) ⇒
+  ∀x. mayloop R x ⇔ mustloop R x
 Proof
-  strip_tac >> Induct_on ‘RTC’ >> rpt strip_tac
-  >- metis_tac[] >>
-  gs[simulates_def, triR_def] >> rename [‘nf sR s’, ‘sR s0 s0'’] >>
-  ‘∃t tT. tR꙳ t0 tT ∧ simR s0' t ∧ tR꙳ t tT’ by metis_tac[] >>
-  ‘∃tt. tR꙳ t tt ∧ simR s tt ∧ nf tR tt’ by metis_tac[] >>
-  ‘∃d. tR꙳ tT d ∧ tR꙳ tt d’ by metis_tac[CR_def, diamond_def] >>
-  qexists_tac ‘tt’ >> simp[] >>
-  ‘tt = d’ by metis_tac[RTC_CASES1, nf_def] >>
-  metis_tac[RTC_CASES_RTC_TWICE]
+  metis_tac[nf_def, mustloop_def, det_term_xor_mayloop]
 QED
 
+        (*
+Theorem TC_mayloop[simp]:
+  mayloop R⁺ x ⇔ mayloop R x
+Proof
+  eq_tac
+  >- (qid_spec_tac ‘x’ >> ho_match_mp_tac mayloop_coind >>
+      simp[Once mayloop_cases, SimpL “$==>”] >> simp[PULL_EXISTS] >>
+      simp[Once TC_CASES2, PULL_EXISTS, DISJ_IMP_THM, LEFT_AND_OVER_OR,
+           FORALL_AND_THM] >> metis_tac[]
+      >- metis_tac[] >>
+      rename [‘R x y’, ‘R⁺ y t’] >> qexists_tac ‘y’ >> simp[] >>
+      simp[Once mayloop_cases]) >>
+  qid_spec_tac ‘x’ >> ho_match_mp_tac mayloop_coind >>
+  metis_tac[TC_CASES1, mayloop_cases]
+QED
+
+Definition forward_sim_def:
+  forward_sim sim sR tR ⇔
+    ∃R. WF R ∧
+        ∀s0 s t0.
+          sim s0 t0 ∧ sR s0 s ⇒
+          (∃t. tR t0 t ∧ sim s t) ∨ sim s t0 ∧ R s s0
+End
+
+Theorem mayloop_WFP:
+  mayloop R x ⇔ ¬WFP Rᵀ x
+Proof
+  eq_tac
+  >- (‘!x. WFP Rᵀ x ⇒ ¬mayloop R x’ suffices_by metis_tac[] >>
+      ho_match_mp_tac WFP_STRONG_INDUCT >> simp[] >> rw[] >>
+      simp[Once mayloop_cases] >> metis_tac[]) >>
+  qid_spec_tac ‘x’ >> ho_match_mp_tac mayloop_coind >>
+  simp[SimpL “$==>”, Once WFP_CASES] >> metis_tac[]
+QED
+
+Definition nf_matching_def:
+  nf_matching sim sR tR ⇔
+    ∀s t. nf sR s ∧ sim s t ⇒ ¬mayloop tR t
+End
+
+Definition postcloudR_def:
+  postcloudR simR sR tR t s ⇔
+    simR s t ∨
+    ∃t0. simR s t0 ∧ tR⁺ t0 t ∧
+         ∀t' s'. tR⁺ t0 t' ∧ tR⁺ t' t ⇒ ¬simR s' t'
+End
+
+Theorem forward_sim_TCinduce:
+  forward_sim sim sR tR ⇒
+  ∀s0 t0.
+    sim s0 t0 ⇒
+    WFP sRᵀ s0 ∧
+    (∃s. sR꙳ s0 s ∧ sim s t0 ∧ nf sR s ∧ ∀s'. sR꙳ s0 s' ⇒ sim s' t0)
+      ∨
+    ∃s t. sR⁺ s0 s ∧ tR t0 t ∧ sim s t
+Proof
+  simp[forward_sim_def] >> rw[] >>
+  qpat_x_assum ‘sim s0 t0’ mp_tac >>
+  map_every qid_spec_tac [‘t0’, ‘s0’] >>
+  drule WF_INDUCTION_THM >>
+  disch_then (assume_tac o SRULE[RIGHT_FORALL_IMP_THM]) >>
+  pop_assum ho_match_mp_tac >> rw[] >>
+  Cases_on ‘∃s'. sR s0 s'’ >> gs[]
+  >- (‘(∃t'. tR t0 t' ∧ sim s' t') ∨ sim s' t0 ∧ R s' s0’ by metis_tac[]
+      >- metis_tac[TC_SUBSET] >>
+      first_assum (drule_all_then strip_assume_tac)
+      >- (Cases_on ‘∃s t. sR⁺ s0 s ∧ tR t0 t ∧ sim s t’ >> gs[] >>
+          disj1_tac >> conj_tac
+          >- (irule WFP_RULES >> simp[] >> qx_gen_tac ‘s1’ >> strip_tac >>
+              ‘sim s1 t0 ∧ R s1 s0’ by metis_tac[TC_SUBSET] >>
+              first_assum
+                (fn th => first_x_assum
+                            (fn ith => mp_then (Pos hd) mp_tac ith th)) >>
+              disch_then $ drule_then strip_assume_tac >>
+              metis_tac[TC_CASES1]) >>
+          irule_at (Pos hd) (cj 2 RTC_RULES) >>
+          first_assum $ irule_at (Pos hd) >>
+          first_assum $ irule_at (Pos hd) >>
+          simp[] >>
+          simp[Once RTC_CASES1, DISJ_IMP_THM, FORALL_AND_THM, PULL_EXISTS] >>
+          qx_genl_tac [‘ss’, ‘s1’] >> strip_tac >>
+          ‘sim s1 t0 ∧ R s1 s0’ by metis_tac[TC_SUBSET] >>
+          first_assum
+            (fn th => first_x_assum
+                        (fn ith => mp_then (Pos hd) mp_tac ith th)) >>
+          disch_then $ drule_then strip_assume_tac >- metis_tac[] >>
+          metis_tac[TC_CASES1]) >>
+      metis_tac[TC_CASES1]) >>
+  ‘∀s. sR꙳ s0 s ⇔ s = s0’ by metis_tac[RTC_CASES1] >> gs[] >>
+  disj1_tac >> simp[nf_def] >> irule WFP_RULES >> simp[]
+QED
+
+Definition tterm_def:
+  tterm sim sR tR t1 t0 ⇔
+    tR t0 t1 ∧ forward_sim sim sR tR⁺ ∧ nf_matching sim sR tR ∧
+    (∀t0 t1 t2. tR t0 t1 ∧ tR t0 t2 ⇒ t1 = t2) ∧
+    ∃t00 s0. sim s0 t00 ∧ tR꙳ t00 t1 ∧
+             ∀t'. tR⁺ t00 t' ∧ tR꙳ t' t1 ⇒
+                  ∀s. sim s t' ⇒ ¬sR꙳ s0 s
+End
+
+Theorem WFP_RTC_along:
+  ∀y x. WFP R y ∧ R꙳ x y ⇒ WFP R x
+Proof
+  Induct_on ‘WFP’ using WFP_STRONG_INDUCT >> rw[] >>
+  qpat_x_assum ‘RTC R x y’ mp_tac >> simp[Once RTC_CASES2] >>
+  metis_tac[]
+QED
+
+Theorem iterator_mayloop:
+  (∀a. a ∈ P ⇒ it a ∈ P) ∧ (∀a b. a ∈ P ⇒ (R a b ⇔ b = it a)) ∧ x ∈ P ⇒
+  mayloop R x
+Proof
+  strip_tac >> qpat_x_assum ‘x ∈ P’ mp_tac >> qid_spec_tac ‘x’ >>
+  ho_match_mp_tac mayloop_coind >> metis_tac[]
+QED
+
+Theorem det_NRC_TC_lemma:
+  (∀a b c. R a b ∧ R a c ⇒ b = c) ⇒
+  NRC R n x y ∧ R⁺ x z ⇒
+  (∃m. m < n ∧ NRC R m z y) ∨ R⁺ y z
+Proof
+  strip_tac >> map_every qid_spec_tac [‘n’, ‘x’, ‘y’, ‘z’] >>
+  Induct_on ‘n’ >> simp[NRC, PULL_EXISTS] >> rpt gen_tac >>
+  simp[SimpL “$==>”, Once TC_CASES1] >> strip_tac
+  >- metis_tac[prim_recTheory.LESS_SUC_REFL] >>
+  rename [‘NRC R n z1 y’, ‘R x z1’, ‘R x z2’, ‘R⁺ z2 z’] >>
+  ‘z1 = z2’ by metis_tac[] >> (* gvs BUG *) pop_assum SUBST_ALL_TAC >>
+  first_x_assum drule_all >> strip_tac >> simp[] >>
+  rename [‘m < n’] >> disj1_tac >> qexists_tac ‘m’ >> simp[]
+QED
+
+Theorem forward_sim_overtakes_tR:
+  (∀t0 t1 t2. tR t0 t1 ∧ tR t0 t2 ⇒ t1 = t2) ∧
+  forward_sim sim sR tR⁺ ∧ nf_matching sim sR tR ⇒
+  sim s0 t0 ∧ tR꙳ t0 w ⇒
+  (∃s t. sR⁺ s0 s ∧ tR꙳ w t ∧ sim s t) ∨
+  WFP tRᵀ w
+Proof
+  strip_tac >> simp[SimpL “$==>”, RTC_eq_NRC] >>
+  simp[PULL_EXISTS] >> map_every qid_spec_tac [‘s0’, ‘t0’] >>
+  completeInduct_on ‘n’ >> rpt strip_tac >>
+  drule_then (drule_then strip_assume_tac) forward_sim_TCinduce
+  >- (rename [‘nf sR s’] >>
+      ‘¬mayloop tR t0’ by metis_tac[nf_matching_def] >>
+      gs[mayloop_WFP] >> disj2_tac >>
+      irule WFP_RTC_along >> simp[inv_MOVES_OUT] >>
+      metis_tac[RTC_eq_NRC]) >>
+  drule_all_then strip_assume_tac det_NRC_TC_lemma
+  >- (first_x_assum $ drule_all_then strip_assume_tac
+      >- metis_tac[TC_RULES] >>
+      simp[]) >>
+  metis_tac[TC_RTC]
+QED
+(*
+Theorem WF_tterm[simp]:
+  WF (tterm sim sR tR)
+Proof
+  simp[WF_DEF, tterm_def] >>
+  Cases_on ‘forward_sim sim sR tR⁺’ >> simp[] >>
+  Cases_on ‘nf_matching sim sR tR’ >> simp[PULL_EXISTS] >>
+  Cases_on ‘∀t0 t1 t2. tR t0 t1 ∧ tR t0 t2 ⇒ t1 = t2’ >> simp[] >>
+  qx_gen_tac ‘tSet’ >> qx_gen_tac ‘w’ >> strip_tac >>
+  ‘∀x. tSet x ⇔ x ∈ tSet’ by simp[IN_DEF] >>
+  pop_assum (gs o single) >>
+  Cases_on ‘∃d. d ∈ tSet ∧ ∀d'. tR d d' ⇒ d' ∉ tSet’ >> gs[]
+  >- (qexists_tac ‘d’ >> simp[]) >>
+  pop_assum (fn th => ‘∀d. d ∈ tSet ⇒ ∃d'. tR d d' ∧ d' ∈ tSet’
+               by metis_tac[th]) >>
+  pop_assum (qx_choose_then ‘next’ strip_assume_tac o
+             SRULE [SKOLEM_THM, GSYM RIGHT_EXISTS_IMP_THM]) >>
+  ‘∀d e. d ∈ tSet ⇒ (tR d e ⇔ e = next d)’ by metis_tac[] >>
+  csimp[] >>
+  Cases_on ‘∀t s. tR꙳ w t ⇒ ¬sim s t’ >> gs[]
+  >- (Cases_on ‘∃t0 s0. tR꙳ t0 w ∧ sim s0 t0’ >> gs[]
+      >- (drule_all_then strip_assume_tac forward_sim_overtakes_tR
+          >- metis_tac[] >>
+          ‘mayloop tR w’ by metis_tac[iterator_mayloop] >>
+          gs[mayloop_WFP]) >>
+      pop_assum (fn th => ‘∀t0 s0. tR꙳ t0 w ⇒ ¬sim s0 t0’ by metis_tac[th]) >>
+      qexists_tac ‘w’ >> simp[] >> qx_genl_tac [‘t0’, ‘s0’] >>
+      Cases_on ‘sim s0 t0’ >> simp[] >>
+      Cases_on ‘tR꙳ t0 (next w)’ >> simp[PULL_EXISTS] >>
+      drule_all_then strip_assume_tac forward_sim_overtakes_tR
+      >- (rename [‘tR꙳ (next w) t’, ‘sim s t’] >>
+          ‘tR w (next w)’ by simp[] >> metis_tac[RTC_RULES]) >>
+      ‘tRᵀ (next w) w’ by simp[] >>
+      ‘WFP tRᵀ w’ by (irule WFP_RULES >> simp[]) >>
+      ‘mayloop tR w’ by metis_tac[iterator_mayloop] >> gs[mayloop_WFP]) >>
 
 
 
+
+  Cases_on ‘∃t. tR꙳ w t ∧ ’
+  Cases_on ‘∀s t. t ∈ tSet ⇒ ¬sim s t’ >> gs[]
+  >- (qexists_tac ‘w’ >> rpt strip_tac >> simp[] >>
+  reverse (Cases_on ‘∀t. t ∈ tSet ⇒ ∃t0 s0. tR꙳ t0 t ∧ sim s0 t0’) >> gs[]
+  >- (qexists_tac ‘t’ >> simp[] >> metis_tac[cj 2 RTC_RULES_RIGHT1]
+
+Theorem detforward_imp_backward:
+  (∀t0 t1 t2. tR t0 t1 ∧ tR t0 t2 ⇒ t1 = t2) ∧
+  nf_matching sim sR tR ∧
+  forward_sim sim sR tR⁺ ⇒
+  ∃sim'. sim ⊆ᵣ sim' ∧ forward_sim sim'ᵀ tR sR⁺
+Proof
+  simp[nf_matching_def] >> strip_tac >> simp[PULL_EXISTS] >>
+  qexists_tac ‘(postcloudR sim sR tR)ᵀ’ >> simp[] >> conj_tac
+  >- simp[RSUBSET,postcloudR_def] >>
+  simp[forward_sim_def, postcloudR_def] >>
+  qexists_tac ‘tterm sim sR tR’ >> rw[]
+
+    [‘postcloudR sim sR tR t0 s0’, ‘tR t0 t1’]
+  >- (gs[postcloudR_def]
+      >- (rename [‘tterm sim sR tR t1 t0’, ‘tR t0 t1’, ‘sim s0 t0’] >>
+
+
+
+
+
+*)
+*)
 val _ = export_theory();
